Add top level backward simulation

src/Compiler.v
@@ -16,6 +16,8 @@
  * along with this program.  If not, see <https://www.gnu.org/licenses/>.
  *)
 
+From coqup Require Import HTLgenproof.
+
 From compcert.common Require Import
     Errors
     Linking.
@@ -49,8 +51,9 @@ From coqup Require
      Verilog
      Veriloggen
      Veriloggenproof
-     HTLgen
-     HTLgenproof.
+     HTLgen.
+
+From compcert Require Import Smallstep.
 
 Parameter print_RTL: Z -> RTL.program -> unit.
 Parameter print_HTL: HTL.program -> unit.
@@ -85,7 +88,9 @@ Definition transf_backend (r : RTL.program) : res Verilog.program :=
   @@ print print_HTL
   @@ Veriloggen.transl_program.
 
-Definition transf_frontend (p: Csyntax.program) : res RTL.program :=
+Check mkpass.
+
+Definition transf_hls (p : Csyntax.program) : res Verilog.program :=
   OK p
   @@@ SimplExpr.transl_program
   @@@ SimplLocals.transf_program
@@ -93,11 +98,6 @@ Definition transf_frontend (p: Csyntax.program) : res RTL.program :=
   @@@ Cminorgen.transl_program
   @@@ Selection.sel_program
   @@@ RTLgen.transl_program
-  @@ print (print_RTL 0).
-
-Definition transf_hls (p : Csyntax.program) : res Verilog.program :=
-  OK p
-  @@@ transf_frontend
   @@@ transf_backend.
 
 Local Open Scope linking_scope.
@@ -110,27 +110,30 @@ Definition CompCert's_passes :=
   ::: mkpass Selectionproof.match_prog
   ::: mkpass RTLgenproof.match_prog
   ::: mkpass Inliningproof.match_prog
-  ::: mkpass HTLgenproof.match_prog
+  ::: (@mkpass _ _ HTLgenproof.match_prog (HTLgenproof.TransfHTLLink HTLgen.transl_program))
   ::: mkpass Veriloggenproof.match_prog
   ::: pass_nil _.
 
-Definition match_prog: Csyntax.program -> RTL.program -> Prop :=
+Definition match_prog: Csyntax.program -> Verilog.program -> Prop :=
   pass_match (compose_passes CompCert's_passes).
 
-Theorem transf_frontend_match:
+Theorem transf_hls_match:
   forall p tp,
-    transf_frontend p = OK tp ->
+    transf_hls p = OK tp ->
     match_prog p tp.
 Proof.
   intros p tp T.
-  unfold transf_frontend in T. simpl in T.
+  unfold transf_hls in T. simpl in T.
   destruct (SimplExpr.transl_program p) as [p1|e] eqn:P1; simpl in T; try discriminate.
   destruct (SimplLocals.transf_program p1) as [p2|e] eqn:P2; simpl in T; try discriminate.
   destruct (Cshmgen.transl_program p2) as [p3|e] eqn:P3; simpl in T; try discriminate.
   destruct (Cminorgen.transl_program p3) as [p4|e] eqn:P4; simpl in T; try discriminate.
   destruct (Selection.sel_program p4) as [p5|e] eqn:P5; simpl in T; try discriminate.
-  rewrite ! compose_print_identity in T.
   destruct (RTLgen.transl_program p5) as [p6|e] eqn:P6; simpl in T; try discriminate.
+  unfold transf_backend in T. simpl in T. rewrite ! compose_print_identity in T.
+  destruct (Inlining.transf_program p6) as [p7|e] eqn:P7; simpl in T; try discriminate.
+  destruct (HTLgen.transl_program p7) as [p8|e] eqn:P8; simpl in T; try discriminate.
+  set (p9 := Veriloggen.transl_program p8) in *.
   unfold match_prog; simpl.
   exists p1; split. apply SimplExprproof.transf_program_match; auto.
   exists p2; split. apply SimplLocalsproof.match_transf_program; auto.
@@ -138,5 +141,99 @@ Proof.
   exists p4; split. apply Cminorgenproof.transf_program_match; auto.
   exists p5; split. apply Selectionproof.transf_program_match; auto.
   exists p6; split. apply RTLgenproof.transf_program_match; auto.
-  inversion T. reflexivity.
+  exists p7; split. apply Inliningproof.transf_program_match; auto.
+  exists p8; split. apply HTLgenproof.transf_program_match; auto.
+  exists p9; split. apply Veriloggenproof.transf_program_match; auto.
+  inv T. reflexivity.
+Qed.
+
+Remark forward_simulation_identity:
+  forall sem, forward_simulation sem sem.
+Proof.
+  intros. apply forward_simulation_step with (fun s1 s2 => s2 = s1); intros.
+- auto.
+- exists s1; auto.
+- subst s2; auto.
+- subst s2. exists s1'; auto.
+Qed.
+
+Theorem cstrategy_semantic_preservation:
+  forall p tp,
+  match_prog p tp ->
+  forward_simulation (Cstrategy.semantics p) (Verilog.semantics tp)
+  /\ backward_simulation (atomic (Cstrategy.semantics p)) (Verilog.semantics tp).
+Proof.
+  intros p tp M. unfold match_prog, pass_match in M; simpl in M.
+Ltac DestructM :=
+  match goal with
+    [ H: exists p, _ /\ _ |- _ ] =>
+      let p := fresh "p" in let M := fresh "M" in let MM := fresh "MM" in
+      destruct H as (p & M & MM); clear H
+  end.
+  repeat DestructM. subst tp.
+  assert (F: forward_simulation (Cstrategy.semantics p) (Verilog.semantics p9)).
+  {
+  eapply compose_forward_simulations.
+    eapply SimplExprproof.transl_program_correct; eassumption.
+  eapply compose_forward_simulations.
+    eapply SimplLocalsproof.transf_program_correct; eassumption.
+  eapply compose_forward_simulations.
+    eapply Cshmgenproof.transl_program_correct; eassumption.
+  eapply compose_forward_simulations.
+    eapply Cminorgenproof.transl_program_correct; eassumption.
+  eapply compose_forward_simulations.
+    eapply Selectionproof.transf_program_correct; eassumption.
+  eapply compose_forward_simulations.
+    eapply RTLgenproof.transf_program_correct; eassumption.
+  eapply compose_forward_simulations.
+    eapply Inliningproof.transf_program_correct; eassumption.
+  eapply compose_forward_simulations.
+    eapply HTLgenproof.transf_program_correct. eassumption.
+  eapply Veriloggenproof.transf_program_correct; eassumption.
+  }
+  split. auto.
+  apply forward_to_backward_simulation.
+  apply factor_forward_simulation. auto. eapply sd_traces. eapply Verilog.semantics_determinate.
+  apply atomic_receptive. apply Cstrategy.semantics_strongly_receptive.
+  apply Verilog.semantics_determinate.
+Qed.
+
+Theorem c_semantic_preservation:
+  forall p tp,
+  match_prog p tp ->
+  backward_simulation (Csem.semantics p) (Verilog.semantics tp).
+Proof.
+  intros.
+  apply compose_backward_simulation with (atomic (Cstrategy.semantics p)).
+  eapply sd_traces; eapply Verilog.semantics_determinate.
+  apply factor_backward_simulation.
+  apply Cstrategy.strategy_simulation.
+  apply Csem.semantics_single_events.
+  eapply ssr_well_behaved; eapply Cstrategy.semantics_strongly_receptive.
+  exact (proj2 (cstrategy_semantic_preservation _ _ H)).
+Qed.
+
+Theorem transf_c_program_correct:
+  forall p tp,
+  transf_hls p = OK tp ->
+  backward_simulation (Csem.semantics p) (Verilog.semantics tp).
+Proof.
+  intros. apply c_semantic_preservation. apply transf_hls_match; auto.
+Qed.
+
+Theorem separate_transf_c_program_correct:
+  forall c_units asm_units c_program,
+  nlist_forall2 (fun cu tcu => transf_hls cu = OK tcu) c_units asm_units ->
+  link_list c_units = Some c_program ->
+  exists asm_program,
+      link_list asm_units = Some asm_program
+   /\ backward_simulation (Csem.semantics c_program) (Verilog.semantics asm_program).
+Proof.
+  intros.
+  assert (nlist_forall2 match_prog c_units asm_units).
+  { eapply nlist_forall2_imply. eauto. simpl; intros. apply transf_hls_match; auto. }
+  assert (exists asm_program, link_list asm_units = Some asm_program /\ match_prog c_program asm_program).
+  { eapply link_list_compose_passes; eauto. }
+  destruct H2 as (asm_program & P & Q).
+  exists asm_program; split; auto. apply c_semantic_preservation; auto.
 Qed.
